\documentclass{article}
\usepackage{ifthen}
\usepackage{epsfig}
\usepackage[utf8]{inputenc}
\usepackage{xcolor}
\color{white}
\pagecolor{black}
\usepackage{newunicodechar}
  \makeatletter
    \def\doxynewunicodechar#1#2{%
    \@tempswafalse
    \edef\nuc@tempa{\detokenize{#1}}%
    \if\relax\nuc@tempa\relax
      \nuc@emptyargerr
    \else
      \edef\@tempb{\expandafter\@car\nuc@tempa\@nil}%
      \nuc@check
      \if@tempswa
        \@namedef{u8:\nuc@tempa}{#2}%
      \fi
    \fi
  }
  \makeatother
  \doxynewunicodechar{⁻}{${}^{-}$}% Superscript minus
  \doxynewunicodechar{²}{${}^{2}$}% Superscript two
  \doxynewunicodechar{³}{${}^{3}$}% Superscript three

\pagestyle{empty}
\begin{document}
$\frac{\exp(a)}{\exp(a)+\exp(b)}$
\pagebreak

$\log\left(\exp(a) + \exp(b)\right)$
\pagebreak

$m_{I\to i}(x_i)$
\pagebreak

$I$
\pagebreak

$i$
\pagebreak

\[ m_{I\to i}(x_i) \propto \sum_{x_{N_I\setminus\{i\}}} f_I(x_I) \prod_{j\in N_I\setminus\{i\}} \prod_{J\in N_j\setminus\{I\}} m_{J\to j}\]
\pagebreak

\[ m_{I\to i}(x_i) \propto \max_{x_{N_I\setminus\{i\}}} f_I(x_I) \prod_{j\in N_I\setminus\{i\}} \prod_{J\in N_j\setminus\{I\}} m_{J\to j}\]
\pagebreak

\[ b_i(x_i) \propto \prod_{I\in N_i} m_{I\to i}(x_i)\]
\pagebreak

\[ b_I(x_I) \propto f_I(x_I) \prod_{j\in N_I} \prod_{J\in N_j\setminus\{I\}} m_{J\to j}(x_j) \]
\pagebreak

\[ \log Z = \sum_i (1 - |N_i|) \sum_{x_i} b_i(x_i) \log b_i(x_i) - \sum_I \sum_{x_I} b_I(x_I) \log \frac{b_I(x_I)}{f_I(x_I)} \]
\pagebreak

$ x_i $
\pagebreak

$ x_i^* $
\pagebreak

$ x_i = x_i^* $
\pagebreak

$\delta_{x_i, x}$
\pagebreak

\[ P(\mathbf{x}) = \prod_{i\in\mathcal{V}} P(x_i \,|\, x_{\mathrm{pa}(i)}) \]
\pagebreak

$\mathrm{pa}(i)$
\pagebreak

\[ P(\mathbf{x}) = \frac{1}{Z} \prod_{C\in\mathcal{C}} \psi_C(x_C) \]
\pagebreak

$ \mathcal{C} $
\pagebreak

$ \psi_C(x_C) $
\pagebreak

$ Z $
\pagebreak

\[ P(\mathbf{x}) = \frac{1}{Z} \prod_{I\in \mathcal{F}} f_I(x_I) \]
\pagebreak

$ \mathcal{F} $
\pagebreak

$ f_I(x_I) $
\pagebreak

$\{x_i\}_{i\in\mathcal{V}}$
\pagebreak

$\{f_I(x_I)\}_{I\in\mathcal{F}}$
\pagebreak

\[ Z = \sum_{\mathbf{x}_{\mathcal{V}}} \prod_{I \in \mathcal{F}} f_I(x_I) \]
\pagebreak

$\{x_i\}_{i\in A}$
\pagebreak

\[ P(\mathbf{x}_{A}) = \frac{1}{Z} \sum_{\mathbf{x}_{\mathcal{V}\setminus A}} \prod_{I \in \mathcal{F}} f_I(x_I) \]
\pagebreak

\[ \mathrm{argmax}_{\mathbf{x}}\,\prod_{I\in\mathcal{F}} f_I(x_I) \]
\pagebreak

$l$
\pagebreak

$x_l$
\pagebreak

$S_{x_l}$
\pagebreak

$S_l$
\pagebreak

$X_l := \{0,1,\dots,S_l-1\}$
\pagebreak

$A := \{x_{l_1},x_{l_2},\dots,x_{l_n}\}$
\pagebreak

$l_1 < l_2$
\pagebreak

$x_{l_1}$
\pagebreak

$x_{l_2}$
\pagebreak

$(l_i)_{i=1}^n$
\pagebreak

$l_1 < l_2 < \dots < l_n$
\pagebreak

$ \prod_{i=1}^n X_{l_i}$
\pagebreak

$(s_1,s_2,\dots,s_n)$
\pagebreak

$x_{l_1} = s_1, \dots, x_{l_n} = s_n$
\pagebreak

\[
  s := \sum_{i=1}^n s_i \prod_{j=1}^{i-1} S_{l_j} 
     = s_1 + s_2 S_{l_1} + s_3 S_{l_1} S_{l_2} + \dots + s_n S_{l_1} \cdots S_{l_{n-1}}.
\]
\pagebreak

$s_i$
\pagebreak

$x_{l_i}$
\pagebreak

\[
  s_i = \left\lfloor\frac{s \mbox { mod } \prod_{j=1}^i S_{l_j}}{\prod_{j=1}^{i-1} S_{l_j}}\right\rfloor.
\]
\pagebreak

$\prod_{i=1}^n S_{l_i}$
\pagebreak

\[
\begin{array}{ccc|c}
x_4 & x_8 & x_7 & \mbox{value}\\
\hline
 0 & 0 & 0  &  0.1\\
 1 & 0 & 0  &  3.5\\
 2 & 0 & 0  &  2.8\\
 0 & 1 & 0  &  6.3\\
 1 & 1 & 0  &  8.4\\
 2 & 1 & 0  &  0.0\\
 0 & 0 & 1  &  7.4\\
 1 & 0 & 1  &  2.4\\
 2 & 0 & 1  &  8.9\\
 0 & 1 & 1  &  1.3\\
 1 & 1 & 1  &  1.6\\
 2 & 1 & 1  &  2.6
\end{array}
\]
\pagebreak

$x_4$
\pagebreak

$x_8$
\pagebreak

$x_7$
\pagebreak

$x_4 x_7 x_8$
\pagebreak

\[
\begin{array}{ccc|c}
x_4 & x_7 & x_8 & \mbox{value}\\
\hline
 0 & 0 & 0  &  0.1\\
 1 & 0 & 0  &  3.5\\
 2 & 0 & 0  &  2.8\\
 0 & 1 & 0  &  7.4\\
 1 & 1 & 0  &  2.4\\
 2 & 1 & 0  &  8.9\\
 0 & 0 & 1  &  6.3\\
 1 & 0 & 1  &  8.4\\
 2 & 0 & 1  &  0.0\\
 0 & 1 & 1  &  1.3\\
 1 & 1 & 1  &  1.6\\
 2 & 1 & 1  &  2.6
\end{array}
\]
\pagebreak

$x_1 = 0, x_3 = 0, x_2 = 1$
\pagebreak

$x_1 = 1, x_3 = 0, x_2 = 1$
\pagebreak

$x_1 = 1, x_2 = 1$
\pagebreak

$x_3$
\pagebreak

$ P( X | Y ) $
\pagebreak

$ | X | $
\pagebreak

$ |X| \cdot |Y| $
\pagebreak

$ P(X | Y=y) $
\pagebreak

$ \frac{\log(Z_t) - \log(Z_{t-1})}{| \log(Z_{t-1}) | } < \mathrm{tol} $
\pagebreak

$X_l = \{0,1,\dots,S_l-1\}$
\pagebreak

$\{x_l\}_{l\in L}$
\pagebreak

$f_L : \prod_{l\in L} X_l \to [0,\infty)$
\pagebreak

$\prod_{l\in L} X_l$
\pagebreak

$\{0,1,\dots,\prod_{l\in L} S_l-1\}$
\pagebreak

$\sigma$
\pagebreak

$ \exp(hx) $
\pagebreak

$ x = \pm 1 $
\pagebreak

$ \exp(J x_1 x_2) $
\pagebreak

$ x_1, x_2 = \pm 1 $
\pagebreak

$ \exp( J \delta_{x_1, x_2} ) $
\pagebreak

$\prod_{l\in L} S_l$
\pagebreak

$-\sum_i p_i \log p_i$
\pagebreak

$1/n$
\pagebreak

$f : \prod_{l\in L} X_l \to [0,\infty)$
\pagebreak

$g : \prod_{m\in M} X_m \to [0,\infty)$
\pagebreak

\[f+g : \prod_{l\in L\cup M} X_l \to [0,\infty) : x \mapsto f(x_L) + g(x_M).\]
\pagebreak

\[f-g : \prod_{l\in L\cup M} X_l \to [0,\infty) : x \mapsto f(x_L) - g(x_M).\]
\pagebreak

\[fg : \prod_{l\in L\cup M} X_l \to [0,\infty) : x \mapsto f(x_L) g(x_M).\]
\pagebreak

\[\frac{f}{g} : \prod_{l\in L\cup M} X_l \to [0,\infty) : x \mapsto \frac{f(x_L)}{g(x_M)}.\]
\pagebreak

$M \subset L$
\pagebreak

$s$
\pagebreak

$x_m$
\pagebreak

$m\in M$
\pagebreak

$s(x_m) \in X_m$
\pagebreak

$g : \prod_{l \in L \setminus M} X_l \to [0,\infty)$
\pagebreak

$g(\{x_l\}_{l\in L \setminus M}) = f(\{x_l\}_{l\in L \setminus M}, \{s(x_m)\}_{m\in M})$
\pagebreak

$L \subset M$
\pagebreak

$g : \prod_{m\in M} X_m \to [0,\infty) : x \mapsto f(x_L)$
\pagebreak

$N$
\pagebreak

$x_0,x_1,\dots,x_{N-1}$
\pagebreak

$M$
\pagebreak

\[
  P(x_0,x_1,\dots,x_{N-1}) = \frac{1}{Z} \prod_{I=0}^{M-1} f_I(x_I), \qquad
  Z = \sum_{x_0}\dots\sum_{x_{N-1}} \prod_{I=0}^{M-1} f_I(X_I).
\]
\pagebreak

$f_I$
\pagebreak

$X_I \subset \{x_0,x_1,\dots,x_{N-1}\}$
\pagebreak

$\min_q KL(p||q)$
\pagebreak

$ KL(q||p) $
\pagebreak

$ c_I $
\pagebreak

$ \alpha=1/c_I $
\pagebreak

\[ m_{I\to i}(x_i) \propto \left( \sum_{x_{N_I\setminus\{i\}}} f_I(x_I)^{1/c_I} \prod_{j\in N_I\setminus\{i\}} m_{I\to j}^{1-1/c_I} \prod_{J\in N_j\setminus\{I\}} m_{J\to j} \right)^{c_I} \]
\pagebreak

\[ b_i(x_i) \propto \prod_{I\in N_i} m_{I\to i} \]
\pagebreak

\[ b_I(x_I) \propto f_I(x_I)^{1/c_I} \prod_{j \in N_I} m_{I\to j}^{1-1/c_I} \prod_{J\in N_j\setminus\{I\}} m_{J\to j} \]
\pagebreak

\[ \log Z = \sum_{I} \sum_{x_I} b_I(x_I) \big( \log f_I(x_I) - c_I \log b_I(x_I) \big) + \sum_{i} (c_i - 1) \sum_{x_i} b_i(x_i) \log b_i(x_i) \]
\pagebreak

\[ c_i := \sum_{I \in N_i} c_I \]
\pagebreak

$ \phi^{\setminus i}_I(x_{I \setminus i}) $
\pagebreak

$b_i$
\pagebreak

\[ b_i^{\mathrm{new}}(x_i) \propto \prod_{I\in N_i} \exp \left( \sum_{x_{N_I \setminus \{i\}}} \log f_I(x_I) \prod_{j \in N_I \setminus \{i\}} b_j(x_j) \right) \]
\pagebreak

\[ b_i^{\mathrm{new}}(x_i) \propto \prod_{I\in N_i} \left( \sum_{x_{N_I \setminus \{i\}}} f_I(x_I) \prod_{j \in N_I \setminus \{i\}} b_j(x_j) \right) \]
\pagebreak

$ M^{(i)}_j $
\pagebreak

$ \Omega^{(i)}_{j,l} $
\pagebreak

$ T^{(i)}_A $
\pagebreak

$ A = \{l_1,l_2,\dots\} $
\pagebreak

$ T^{(i)}_j $
\pagebreak

$ \Gamma^{(i)}_{j,l_1l_2} $
\pagebreak

$ \Gamma^{(i)}_{l_1l_2} $
\pagebreak

$\alpha$
\pagebreak

$\beta$
\pagebreak

$x$
\pagebreak

\[\sum_{\alpha \ni x} c_\alpha + \sum_{\beta \ni x} c_\beta = 1\]
\pagebreak

\[ c_\beta := 1 - \sum_{\gamma \in \mathrm{an}(\beta)} c_\gamma \]
\pagebreak

$\mathrm{an}(\beta)$
\pagebreak

$\tilde f_i(x_j,x_k)$
\pagebreak

$\tilde f_i(x_s)$
\pagebreak

\[ m_{I\to i}(x_i) \propto \sum_{x_{N_I\setminus\{i\}}} f_I(x_I)^{1/c_I} \prod_{j\in N_I\setminus\{i\}} m_{I\to j}^{c_I-1} \prod_{J\in N_j\setminus\{I\}} m_{J\to j}^{c_J} \]
\pagebreak

\[ b_i(x_i) \propto \prod_{I\in N_i} m_{I\to i}^{c_I} \]
\pagebreak

\[ b_I(x_I) \propto f_I(x_I)^{1/c_I} \prod_{j \in N_I} m_{I\to j}^{c_I-1} \prod_{J\in N_j\setminus\{I\}} m_{J\to j}^{c_J} \]
\pagebreak

$\ell_1$
\pagebreak

$\ell_\infty$
\pagebreak

$\sum_i p_i (\log p_i - \log q_i)$
\pagebreak

$\frac{1}{2}\sum_i (\sqrt{p_i}-\sqrt{q_i})^2$
\pagebreak

$\{x_{l(0)},x_{l(1)},\dots,x_{l(n-1)}\}$
\pagebreak

$l(0) < l(1) < \dots < l(n-1)$
\pagebreak

$s(x_l) \in \{0,1,\dots,S_l-1\}$
\pagebreak

$s(x_l)=0$
\pagebreak

$S$
\pagebreak

\begin{eqnarray*}
  S &:=& \sum_{i=0}^{n-1} s(x_{l(i)}) \prod_{j=0}^{i-1} S_{l(j)} \\
    &= & s(x_{l(0)}) + s(x_{l(1)}) S_{l(0)} + s(x_{l(2)}) S_{l(0)} S_{l(1)} + \dots + s(x_{l(n-1)}) S_{l(0)} \cdots S_{l(n-2)}.
\end{eqnarray*}
\pagebreak

$l\in L$
\pagebreak

$\sigma : \prod_{l\in L} X_l \to \{0,1,\dots,\prod_{l\in L} S_l-1\}$
\pagebreak

$\sigma^{-1}$
\pagebreak

$s(x_l)$
\pagebreak

\begin{eqnarray*}
  s(x_{l(i)}) = \left\lfloor\frac{S \mbox { mod } \prod_{j=0}^{i} S_{l(j)}}{\prod_{j=0}^{i-1} S_{l(j)}}\right\rfloor \qquad \mbox{for all $i=0,\dots,n-1$}.
\end{eqnarray*}
\pagebreak

$\sigma^{-1} : \{0,1,\dots,\prod_{l\in L} S_l-1\} \to \prod_{l\in L} X_l$
\pagebreak

\end{document}
